Impl.getEntryGE etc.

src/Std/Data/DTreeMap/Internal/Def.lean
@@ -56,4 +56,22 @@ def size : Impl α β → Nat
 @[Std.Internal.tree_tac] theorem size_leaf : (Impl.leaf : Impl α β).size = 0 := rfl
 @[Std.Internal.tree_tac] theorem size_inner {sz k v l r} : (Impl.inner sz k v l r : Impl α β).size = sz := rfl
 
+/-!
+## `toListModel`
+
+`toListModel` is defined here because it is required to define the `Ordered` predicate.
+-/
+
+/--
+Flattens a tree into a list of key-value pairs. This function is defined for verification
+purposes and should not be executed because it is very inefficient.
+-/
+def toListModel : Impl α β → List ((a : α) × β a)
+  | .leaf => []
+  | .inner _ k v l r => l.toListModel ++ ⟨k, v⟩ :: r.toListModel
+
+@[simp] theorem toListModel_leaf : (.leaf : Impl α β).toListModel = [] := rfl
+@[simp] theorem toListModel_inner {sz k v l r} :
+  (.inner sz k v l r : Impl α β).toListModel = l.toListModel ++ ⟨k, v⟩ :: r.toListModel := rfl
+
 end Std.DTreeMap.Internal.Impl
