src/Std/Data/DTreeMap/Internal/WF/Def.lean
@@ -26,18 +26,6 @@ namespace Std.DTreeMap.Internal
 
 namespace Impl
 
-/--
-Flattens a tree into a list of key-value pairs. This function is defined for verification
-purposes and should not be executed because it is very inefficient.
--/
-def toListModel : Impl α β → List ((a : α) × β a)
-  | .leaf => []
-  | .inner _ k v l r => l.toListModel ++ ⟨k, v⟩ :: r.toListModel
-
-/-- The tree map property. -/
-def Ordered [Ord α] (t : Impl α β) : Prop :=
-  t.toListModel.Pairwise (fun a b => compare a.1 b.1 = .lt)
-
 /-- Well-formedness of tree maps. -/
 inductive WF [Ord α] : {β : α → Type v} → Impl α β → Prop where
   /-- This is the actual well-formedness invariant: the tree must be a balanced BST. -/
